thys/Efficient_Weighted_Path_Order/WPO_Mem_Impl.thy
@@ -82,11 +82,11 @@ lemma wpo_mem: fixes rli rri :: "index \<Rightarrow> ('f,'v)term" (* reverse ind
     wpoub: "wpoub = wpo_ub pr prl ssimple large cS cNS \<sigma> c" 
     and wpo: "wpo = (\<lambda> (s,t). wpoub s t)" 
     and ri: "ri = map_prod rli rri"
-    and "\<And> si. fst st \<unrhd> si \<Longrightarrow> rli (index si) = flatten si \<and> stored si = flatten si" 
-    and "\<And> ti. snd st \<unrhd> ti \<Longrightarrow> rri (index ti) = flatten ti \<and> stored ti = flatten ti" 
+    and "\<And> si. fst st \<unrhd> si \<Longrightarrow> rli (index si) = unindex si \<and> stored si = unindex si" 
+    and "\<And> ti. snd st \<unrhd> ti \<Longrightarrow> rri (index ti) = unindex ti \<and> stored ti = unindex ti" 
     and "valid_memory wpo ri m" 
-  shows "wpo_mem m st = (p,m') \<Longrightarrow> p = wpo (map_prod flatten flatten st) \<and> valid_memory wpo ri m'"
-    "wpo_main m st = (p,m') \<Longrightarrow> p = wpo (map_prod flatten flatten st) \<and> valid_memory wpo ri m'"
+  shows "wpo_mem m st = (p,m') \<Longrightarrow> p = wpo (map_prod unindex unindex st) \<and> valid_memory wpo ri m'"
+    "wpo_main m st = (p,m') \<Longrightarrow> p = wpo (map_prod unindex unindex st) \<and> valid_memory wpo ri m'"
   using assms(4-)
 proof (induct m st and m st arbitrary: p m' and p m' rule: wpo_mem_wpo_main.induct)
   case (1 m s t)
@@ -94,7 +94,7 @@ proof (induct m st and m st arbitrary: p m' and p m' rule: wpo_mem_wpo_main.indu
   note revi = 1(3,4)[unfolded fst_conv snd_conv]
   note mem = 1(5)
   note res = 1(2)[unfolded wpo wpo_mem.simps Let_def]
-  have ri: "ri (index s, index t) = (flatten s, flatten t)" 
+  have ri: "ri (index s, index t) = (unindex s, unindex t)" 
     unfolding ri using revi(1)[of s] revi(2)[of t] by auto
   show ?case
   proof (cases "Mapping.lookup m (index s, index t)")
@@ -108,7 +108,7 @@ proof (induct m st and m st arbitrary: p m' and p m' rule: wpo_mem_wpo_main.indu
     case None
     note res = res[unfolded None option.simps]
     obtain res2 mem2 where rec: "wpo_main m (s, t) = (res2, mem2)" by fastforce
-    have res2: "res2 = wpo (flatten s, flatten t)" and mem: "valid_memory wpo ri mem2" 
+    have res2: "res2 = wpo (unindex s, unindex t)" and mem: "valid_memory wpo ri mem2" 
       using IH[OF refl refl None rec revi mem] by auto
     from res[unfolded rec split]
     have p: "p = res2" and m': "m' = Mapping.update (index s, index t) res2 mem2" by auto
@@ -117,15 +117,15 @@ proof (induct m st and m st arbitrary: p m' and p m' rule: wpo_mem_wpo_main.indu
   qed
 next
   case (2 m s t)
-  let ?s = "flatten s" 
-  let ?t = "flatten t" 
+  let ?s = "unindex s" 
+  let ?t = "unindex t" 
   note revi = 2(6,7)[unfolded fst_conv snd_conv]
   from revi(1)[of s] revi(2)[of t]
-  have stored: "stored s = flatten s" "stored t = flatten t" by auto
+  have stored: "stored s = unindex s" "stored t = unindex t" by auto
   note IHs = 2(1-4)[OF stored[symmetric]]
   note mem = 2(8)
   note res = 2(5)[unfolded wpo_main.simps Let_def stored]
-  have wpo_st: "wpo (flatten s, flatten t) = wpoub (flatten s) (flatten t)" for s t  
+  have wpo_st: "wpo (unindex s, unindex t) = wpoub (unindex s) (unindex t)" for s t  
     unfolding wpo by simp
   note wpo = this[of s t,unfolded wpoub wpo_ub.simps[of _ _ _ _ _ _ _ _ ?s ?t], folded wpoub]
   show ?case
@@ -138,24 +138,24 @@ next
     then obtain f i where s: "s = Fun (f,i) ss" by (cases fi, auto)
     let ?Sta = "status \<sigma> (f, length ss)" 
     note res = res[unfolded s term.simps name_of.simps, folded s]
-    note wpo = wpo[unfolded s flatten.simps term.simps, folded flatten.simps[of _ i], folded s, 
+    note wpo = wpo[unfolded s unindex.simps term.simps, folded unindex.simps[of _ i], folded s, 
         unfolded length_map Let_def]
     show ?thesis
     proof (rule ccontr)
       assume neg: "\<not> ?thesis" 
       from neg res mem wpo s have ncS: "\<not> cS ?s ?t" by auto
       from neg res mem wpo s ncS have cNS: "cNS ?s ?t" by (auto split: if_splits)
-      have id: "map_prod flatten flatten (s,t) = (flatten s, flatten t)" for s t :: "('f,'v)indexed_term" by auto
+      have id: "map_prod unindex unindex (s,t) = (unindex s, unindex t)" for s t :: "('f,'v)indexed_term" by auto
       define sss where "sss = map ((!) ss) ?Sta" 
       note IHs = IHs[OF ncS cNS s refl refl refl, unfolded name_of.simps, unfolded id fst_conv snd_conv, folded sss_def]
       from ncS cNS have id: "cS ?s ?t = False" "cNS ?s ?t = True" by auto
       note res = res[unfolded id if_True if_False, folded sss_def]
-      have sss: "(map ((!) (map flatten ss)) ?Sta) = map flatten sss" 
+      have sss: "(map ((!) (map unindex ss)) ?Sta) = map unindex sss" 
         unfolding sss_def by (auto dest: set_status_nth[OF refl])
       note wpo = wpo[unfolded id if_True if_False]
       have sss_sub: "set sss \<subseteq> set ss" unfolding sss_def by (auto dest: set_status_nth[OF refl])
-      let ?cond1' = "Bex (set sss) (\<lambda>s. snd (wpoub (flatten s) (flatten t)))" 
-      let ?cond1'' = "Bex (set ?Sta) (\<lambda>i. snd (wpoub (map flatten ss ! i) (flatten t)))" 
+      let ?cond1' = "Bex (set sss) (\<lambda>s. snd (wpoub (unindex s) (unindex t)))" 
+      let ?cond1'' = "Bex (set ?Sta) (\<lambda>i. snd (wpoub (map unindex ss ! i) (unindex t)))" 
       have "?cond1'' = ?cond1'" unfolding sss_def
         using set_status_nth[OF refl, of _ \<sigma> f ss] by simp
       note wpo = wpo[unfolded this sss]
@@ -165,11 +165,11 @@ next
         fix si
         assume si: "si \<in> set sss" 
         have "wpo_mem m (si, t) = (p, m') \<Longrightarrow>
-            valid_memory wpo ri m \<Longrightarrow> p = wpo (flatten si, flatten t) \<and> valid_memory wpo ri m'" 
+            valid_memory wpo ri m \<Longrightarrow> p = wpo (unindex si, unindex t) \<and> valid_memory wpo ri m'" 
           for m p m'
           by (intro IHs(1)[OF si _ revi, of m p m'], insert sss_sub s si, auto)
       }
-      hence "memoize_fun wpo_mem wpo (map_prod flatten flatten) ri ((\<lambda>s'. (s', t)) ` set sss)" 
+      hence "memoize_fun wpo_mem wpo (map_prod unindex unindex) ri ((\<lambda>s'. (s', t)) ` set sss)" 
         by (intro memoize_funI, auto)
       from exists_mem[OF mem cond1 this]
       have cond1': "?cond1' = b1" and mem1: "valid_memory wpo ri m1" 
@@ -193,20 +193,20 @@ next
         obtain prs prns where pr: "pr ?f ?g = (prs, prns)" by force
         let ?sta = "(status \<sigma> (g, length ts))" 
         define tss where "tss = map ((!) ts) ?sta" 
-        have tss: "(map ((!) (map flatten ts)) ?sta) = map flatten tss" 
+        have tss: "(map ((!) (map unindex ts)) ?sta) = map unindex tss" 
           unfolding tss_def by (auto dest: set_status_nth[OF refl])
         have tss_sub: "set tss \<subseteq> set ts" unfolding tss_def by (auto dest: set_status_nth[OF refl])
         note res = res[unfolded t term.simps name_of.simps pr split, folded tss_def]
-        note wpo = wpo[unfolded t flatten.simps term.simps length_map pr split, 
-            folded flatten.simps[of _ j], folded t, unfolded tss]
+        note wpo = wpo[unfolded t unindex.simps term.simps length_map pr split, 
+            folded unindex.simps[of _ j], folded t, unfolded tss]
         from neg res mem1 wpo have prns: "prns" by (auto split: if_splits)
         note IHs = IHs[OF t refl refl, unfolded name_of.simps, OF refl pr[symmetric], folded tss_def, OF prns]
         have prns: "(prns \<and> b) = b" "prns = True" for b using prns by auto
         note res = res[unfolded prns if_True]
         note wpo = wpo[unfolded prns(1)]
         let ?cond2 = "forall_mem (\<lambda> t'. (s,t')) wpo_mem fst m1 tss" 
-        let ?cond2'' = "Ball (set ?sta) (\<lambda>j. fst (wpoub ?s (map flatten ts ! j)))" 
-        let ?cond2' = "Ball (set tss) (\<lambda>t. fst (wpoub ?s (flatten t)))"
+        let ?cond2'' = "Ball (set ?sta) (\<lambda>j. fst (wpoub ?s (map unindex ts ! j)))" 
+        let ?cond2' = "Ball (set tss) (\<lambda>t. fst (wpoub ?s (unindex t)))"
         have "?cond2'' = ?cond2'" unfolding tss_def
           using set_status_nth[OF refl, of _ \<sigma> g ts] by simp
         note wpo = wpo[unfolded this]
@@ -215,11 +215,11 @@ next
           fix ti
           assume ti: "ti \<in> set tss" 
           have "wpo_mem m (s, ti) = (p, m') \<Longrightarrow>
-            valid_memory wpo ri m \<Longrightarrow> p = wpo (flatten s, flatten ti) \<and> valid_memory wpo ri m'" 
+            valid_memory wpo ri m \<Longrightarrow> p = wpo (unindex s, unindex ti) \<and> valid_memory wpo ri m'" 
             for m p m'
             by (intro IHs(1)[OF ti _ revi, of m p m'], insert tss_sub t ti, auto)
         }
-        hence "memoize_fun wpo_mem wpo (map_prod flatten flatten) ri (Pair s ` set tss)" 
+        hence "memoize_fun wpo_mem wpo (map_prod unindex unindex) ri (Pair s ` set tss)" 
           by (intro memoize_funI, auto)
         from forall_mem[OF mem1 cond2 this]   
         have cond2': "?cond2' = b2" and mem2: "valid_memory wpo ri m2"
@@ -240,7 +240,7 @@ next
           from True have lex: "?is_lex = True" by auto
           note res = res[unfolded lex if_True]
           note wpo = wpo[unfolded lex if_True]
-          have memo: "memoize_fun wpo_mem wpo (map_prod flatten flatten) ri (set sss \<times> set tss)" 
+          have memo: "memoize_fun wpo_mem wpo (map_prod unindex unindex) ri (set sss \<times> set tss)" 
             apply (rule memoize_fun_pairI)
             apply (rule IH)
                  apply force
@@ -249,7 +249,7 @@ next
             subgoal by (rule revi, insert sss_sub, auto simp: s)
             subgoal by (rule revi, insert tss_sub, auto simp: t)
             by auto
-          have "p = lex_ext_unbounded wpoub (map flatten sss) (map flatten tss) \<and> valid_memory wpo ri m'" 
+          have "p = lex_ext_unbounded wpoub (map unindex sss) (map unindex tss) \<and> valid_memory wpo ri m'" 
             by (rule lex_ext_unbounded_mem[OF assms(2) mem2 res memo])
           with res wpo neg
           show ?thesis by auto
@@ -267,7 +267,7 @@ next
             from True have mul: "?is_mul = True" by auto
             note res = res[unfolded mul if_True]
             note wpo = wpo[unfolded mul if_True]
-            have memo: "memoize_fun wpo_mem wpo (map_prod flatten flatten) ri (set sss \<times> set tss)" 
+            have memo: "memoize_fun wpo_mem wpo (map_prod unindex unindex) ri (set sss \<times> set tss)" 
               apply (rule memoize_fun_pairI)
               apply (rule IH)
                    apply force
@@ -276,7 +276,7 @@ next
               subgoal by (rule revi, insert sss_sub, auto simp: s)
               subgoal by (rule revi, insert tss_sub, auto simp: t)
               by auto
-            have "p = mul_ext_impl wpoub (map flatten sss) (map flatten tss) \<and> valid_memory wpo ri m'" 
+            have "p = mul_ext_impl wpoub (map unindex sss) (map unindex tss) \<and> valid_memory wpo ri m'" 
               using mul_ext_mem(1)[OF assms(2) mem2 res memo] by auto
             with res wpo neg 
             show ?thesis unfolding mul_ext_code by auto
@@ -303,11 +303,11 @@ proof -
   let ?m = "Mapping.empty :: term_rel_mem" 
   have m: "valid_memory (\<lambda>(s, t). wpo_ub pr prl ssimple large cS cNS \<sigma> c s t) (map_prod rl rr) ?m" for rl rr
     unfolding valid_memory_def by auto
-  from index_term_index_flatten[of s] obtain f where f: "\<forall>t\<unlhd> index_term s. f (index t) = flatten t \<and> stored t = flatten t" by auto
-  from index_term_index_flatten[of t] obtain g where g: "\<forall>s\<unlhd> index_term t. g (index s) = flatten s \<and> stored s = flatten s" by auto
+  from index_term_index_unindex[of s] obtain f where f: "\<forall>t\<unlhd> index_term s. f (index t) = unindex t \<and> stored t = unindex t" by auto
+  from index_term_index_unindex[of t] obtain g where g: "\<forall>s\<unlhd> index_term t. g (index s) = unindex s \<and> stored s = unindex s" by auto
   obtain p m where res: "wpo_mem ?m (?s,?t) = (p,m)" by fastforce
   hence impl: "wpo_mem_impl s t = p" unfolding wpo_mem_impl_def by simp
-  also have "...   = wpo_ub pr prl ssimple large cS cNS \<sigma> c (flatten (index_term s)) (flatten (index_term t))" 
+  also have "...   = wpo_ub pr prl ssimple large cS cNS \<sigma> c (unindex (index_term s)) (unindex (index_term t))" 
     by (rule wpo_mem(1)[THEN conjunct1, OF refl refl refl _ _ m res, unfolded map_prod_simp split fst_conv snd_conv, of f g])
       (insert f g, auto)
   finally show ?thesis by simp
